Soundness of STLCEx completed.

MoreStlc.v
@@ -1,5 +1,5 @@
 Require Import SfLib.
-
+Require Import LibTactics.
 Require Import Types.
 Require Import Smallstep.
 Require Import Stlc.
@@ -185,7 +185,7 @@ Fixpoint subst (x : id) (s : tm) (org : tm) : tm :=
         | tpred n => tpred ([x := s] n)
         | tmult a b => tmult ([x := s] a) ([x := s] b)
         | tif0 t t0 t1 => tif0 ([x := s] t) ([x := s] t0) ([x := s] t1)
-        | tlet t u v => if(eq_id_dec t x) then org else tlet t u ([x := s] v)
+        | tlet t u v => if(eq_id_dec t x) then tlet t ([x := s] u) v else tlet t ([x := s] u) ([x := s] v)
         | tpair a b => tpair ([ x:= s] a) ([x := s] b)
         | tfst t => tfst ([x := s] t)
         | tsnd t => tsnd ([x := s] t)
@@ -564,10 +564,14 @@ Inductive occurs_free : id -> tm -> Prop :=
             forall i t t0 t1,
                 occurs_free i t1 ->
                 occurs_free i (tif0 t t0 t1)
-    | occurs_free_let :
+    | occurs_free_let0 :
         forall i j x v,
             occurs_free i v ->
             i <> j ->
+            occurs_free i (tlet j x v)
+    | occurs_free_let1 :
+        forall i j x v,
+            occurs_free i x ->
             occurs_free i (tlet j x v)
     | occurs_free_pair0:
         forall i a b,
@@ -628,7 +632,11 @@ Inductive occurs_free : id -> tm -> Prop :=
                 i <> h ->
                 i <> t ->
                 occurs_free i casel ->
-                occurs_free i (lcase l casenil h t casel).
+                occurs_free i (lcase l casenil h t casel)
+    | occurs_free_fix:
+        forall i x,
+            occurs_free i x ->
+            occurs_free i (tfix x).
 
     Hint Constructors occurs_free.
 Theorem occurs_dec :
@@ -655,9 +663,9 @@ Theorem occurs_dec :
     destruct (eq_id_dec ii i); subst. right; intro HH; inversion HH; subst. destruct (H2 eq_refl).
     left; eauto.
     destruct (eq_id_dec ii i); subst. right; intro HH; inversion HH; subst. destruct (H4 eq_refl).
+    eauto.
     left; eauto.
-    destruct (eq_id_dec ii i); subst. right; intro HH; inversion HH; subst. destruct (H4 eq_refl).
-    left; eauto.
+
     destruct (eq_id_dec ii i); destruct (eq_id_dec ii i0); subst; eauto. right; intro HH; inversion HH; subst; eauto.
     destruct (eq_id_dec ii i); destruct (eq_id_dec ii i0); subst; eauto. right; intro HH; inversion HH; subst; eauto. right ; intro HH; inversion HH; subst; eauto.
     destruct (eq_id_dec ii i); destruct (eq_id_dec ii i0); subst; eauto. right; intro HH; inversion HH; subst; eauto. right ; intro HH; inversion HH; subst; eauto.
@@ -751,13 +759,20 @@ Theorem ctx_swap:
     repeat eapply update_inc; auto.
 Qed.
 
+Hint Resolve  occurs_dec contrapositive  : occurs_free_db.
+
+Hint Resolve refl_ctxeq trans_ctxeq ctx_swap update_permute update_shadow : ctx_db.
+
+
 Lemma non_occurs_free_ctx_add:
 forall x i T U G,
     G |= x \in T ->
     ~occurs_free i x ->
     update i U G |= x \in T.
 
-intro x; induction x.
+intro x; induction x;
+try (intros i T U G hh; inversion hh; subst;  eauto 10 with occurs_free_db
+; fail).
 
 intros. eapply tyVar. cbn.
 inversion H; subst. destruct (eq_id_dec i i0); subst; eauto.
@@ -770,8 +785,198 @@ apply refl_ctxeq. assert (occurs_free i0 (tabs i t x)); eauto. destruct (H0 H1).
 eapply ctx_swap. eauto. eapply symm_ctxeq. eapply update_shadow.
 apply refl_ctxeq. eapply ctx_swap. eapply (IHx _ _ _ _ H6 n).
 eapply update_permute; eauto. apply refl_ctxeq.
-(* Tedious. I have to make small lemma into hint base and ..*)
-intros. inversion H; inver
+intros i T U G h1 h2; inversion h1; subst;
+assert (~occurs_free i x1) as hh1; eauto with occurs_free_db;
+assert (~occurs_free i x2) as hh2; eauto with occurs_free_db;
+assert (~occurs_free i x3) as hh3; eauto with occurs_free_db;
+eauto with occurs_free_db.
+
+intros i0 T U G h1 h2; inversion h1; subst; eauto with occurs_free_db; eauto with ctx_db; eauto with occurs_free_db.
+assert (~occurs_free i0 x1) as hh1; eauto with occurs_free_db.
+destruct (eq_id_dec i0 i); subst; eapply tyLet; eauto with ctx_db.
+eapply ctx_swap. apply H4. eapply symm_ctxeq. eapply update_shadow.
+eapply refl_ctxeq. eauto.
+assert (~occurs_free i0 x2); eauto 10 with occurs_free_db.
+forwards : IHx2; eauto 5 with ctx_db. eapply ctx_swap; eauto with ctx_db.
+eapply update_permute; eauto. eapply refl_ctxeq.
+
+intros. assert (~occurs_free i1 x1); eauto with occurs_free_db.
+inversion H; subst. 
+Print has_type.
+eapply tySCase; eauto with occurs_free_db.
+destruct (eq_id_dec i1 i); subst; eauto with ctx_db.
+Print symm_ctxeq.
+eapply ctx_swap;  eauto 10 using symm_ctxeq with ctx_db. eapply symm_ctxeq; eauto with ctx_db.
+eapply update_shadow. eapply refl_ctxeq.
+assert (~occurs_free i1 x2); eauto with occurs_free_db.
+eapply ctx_swap; try eapply update_permute; eauto.
+eapply refl_ctxeq.
+destruct (eq_id_dec i0 i1); subst.
+eapply ctx_swap; eauto using update_shadow.
+eapply symm_ctxeq; eapply update_shadow; eapply refl_ctxeq.
+eapply ctx_swap; try eapply update_permute. 
+eapply IHx3; eauto with occurs_free_db. eauto. eapply refl_ctxeq.
+
+intros. inversion H; subst. eapply tyLCase; eauto with occurs_free_db.
+destruct (eq_id_dec i i1); subst.
+eapply ctx_swap; try eapply update_permute. 
+eapply ctx_swap; try eapply update_inc. eapply ctx_swap ; try eapply update_permute; eauto.
+eapply refl_ctxeq. eapply symm_ctxeq; eapply update_shadow.
+eapply refl_ctxeq. eauto. eapply refl_ctxeq.
+destruct (eq_id_dec i1 i0); subst.
+eapply ctx_swap; try eapply update_inc; eauto.
+eapply symm_ctxeq; eapply update_shadow. eapply refl_ctxeq.
+assert (~occurs_free i1 x3); eauto with occurs_free_db.
+pose (IHx3 _ _ U _ H10 H1).
+assert (update i T0 (update i1 U (update i0 (TList T0) G)) |= x3 \in T).
+eapply ctx_swap; try eapply update_permute; eauto.
+eapply refl_ctxeq.
+eapply ctx_swap; try eapply update_inc; eauto.
+eapply update_permute. eauto. eapply refl_ctxeq.
+
+Qed.
+
+
+Theorem empty_is_strong :
+    forall G t T,
+        empty |= t \in T ->
+        G |= t \in T.
+
+    intro G; induction G; eauto.
+    intros. pose (empty_is_closed _ _ H).
+    unfold closed in *.
+    pose (c i).
+    eapply non_occurs_free_ctx_add; eauto.
+Qed.
+
+Lemma app_preserv:
+    forall t x y T G U,
+        U |= tabs x T t \in TArrow T G ->
+        empty |= y \in T ->
+        U |= [x := y] t \in G.
+
+    intro t; induction t; eauto;
+    cbn; intros x y T G U h1 h2;
+    try (inversion h1; subst;
+    try match goal with
+        | [H1: update _ _ _ |= _ \in _ |- _] =>
+    inversion H1;subst; eauto 10
+    end; fail).
+
+    intros. inversion h1; subst. 
+    unfold subst. inversion H1; subst.
+    cbn in *. 
+    destruct (eq_id_dec i x); destruct (eq_id_dec x i); subst;
+    try match goal with
+        | [H1 : ?x <> ?x |- _] => destruct (H1 eq_refl)
+        end.
+    inversion H2; subst;eauto. eapply empty_is_strong; eauto.
+    eauto.
+
+    cbn; intros. inversion h1; subst. inversion H1; subst.
+    destruct (eq_id_dec i x); subst. eapply tyAbs. eapply ctx_swap; try eapply update_shadow.
+    eauto. eapply refl_ctxeq. eapply tyAbs. eapply IHt; eauto.
+    eapply tyAbs; eapply ctx_swap ; try eapply update_permute; eauto.
+    eapply refl_ctxeq.
+
+    inversion h1; subst. inversion H1; subst.
+    destruct (eq_id_dec i x); subst; eauto 10;
+    eapply tyLet. eapply ctx_swap; try eapply update_shadow; eauto.
+    eapply refl_ctxeq. 
+    eauto. eapply IHt2. eapply tyAbs. eapply ctx_swap; try eapply update_permute; eauto.
+    eapply refl_ctxeq. eapply empty_is_strong; eauto.
+    eapply IHt1; eauto.
+
+    inversion h1; subst. inversion H1; subst; eauto.
+    eapply tySCase; eauto. destruct (eq_id_dec i x); subst.
+    eapply ctx_swap; try eapply update_shadow; eauto. eapply refl_ctxeq.
+    eapply IHt2. eapply tyAbs; eauto. eapply ctx_swap; try eapply update_permute;eauto.
+    eapply refl_ctxeq; eauto. eauto.
+    destruct (eq_id_dec i0 x); subst; eauto. 
+    eapply ctx_swap; try eapply update_shadow; eauto. eapply refl_ctxeq.
+    eapply IHt3; eauto. eapply tyAbs; eauto. eapply ctx_swap; try eapply update_permute; eauto 10.
+    eapply refl_ctxeq.
+
+    inversion h1; subst. inversion H1; subst; eapply tyLCase; destruct (eq_id_dec i x); subst; eauto.
+    eapply ctx_swap; try (eapply symm_ctxeq; eapply update_shadow); eauto.
+    eapply trans_ctxeq. eapply update_inc. eapply update_permute; eauto.
+    eapply refl_ctxeq. eapply update_shadow. eapply refl_ctxeq.
+    destruct (eq_id_dec i0 x); subst. eapply ctx_swap; try eapply update_inc. eapply H9.
+    eapply update_shadow. eapply refl_ctxeq. eapply IHt3. eapply tyAbs.
+    eapply ctx_swap; try eapply H9. eapply trans_ctxeq; try (eapply update_inc; eapply update_permute); eauto.
+    eapply refl_ctxeq. eapply update_permute; eauto. eapply refl_ctxeq. eauto.
+Qed.
+
+Theorem preservation :
+    forall t t' T,
+        empty |= t \in T ->
+        step t t' ->
+        empty |= t' \in T.
+
+    intro t; induction t;
+    try (intros t' T h1 h2; try value_stepping_false; fail);
+    try (intros t' T h1 h2; inversion h1; inversion h2; subst; eauto; fail).
+
+    intros t' T h1 h2; inversion h1; subst; inversion h2; subst; eauto.
+    eapply app_preserv; eauto. inversion H2; subst; eauto.
+
+    intros t' T h1 h2; inversion h1; inversion h2; subst; eauto.
+    eapply app_preserv; eauto.
+
+    intros t' T h1 h2; inversion h1; inversion h2; subst; eauto.
+    inversion H1; subst; eauto.
+    intros t' T h1 h2; inversion h1; inversion h2; subst; eauto.
+    inversion H1; subst; eauto.
+    intros t' T h1 h2; inversion h1; inversion h2; subst; eauto.
+    eapply app_preserv; eauto. inversion H8; eauto.
+    eapply app_preserv; eauto. inversion H8; eauto.
+
+    intros t' T h1 h2; inversion h1; inversion h2; subst; eauto.
+    inversion H9;subst; eauto.
+    eapply app_preserv; eauto. eapply tyAbs. eapply app_preserv; eauto.
+    eapply tyAbs; eauto. eapply ctx_swap; try eapply update_permute; eauto.
+    eapply refl_ctxeq.
+    
+    intros t' T h1 h2; inversion h1; inversion h2; subst; eauto.
+    inversion h1; subst; inversion H1; subst; eauto.
+    eapply app_preserv; eauto.
+Qed.
+
+
+Definition stuck (t: tm) : Prop :=
+(normal_form step) t /\ ~ value t.
+
+Notation "t '==>*' t'" := (multi step t t') (at level 40).
+
+Corollary soundness :
+    forall t t' T,
+        empty |= t \in T ->
+        t ==>* t' ->
+        ~(stuck t').
+
+
+        unfold stuck; unfold not; unfold normal_form; unfold not.
+        intros t t' T h1 h.
+        generalize dependent T.
+        induction h; eauto; try tauto.
+        intros T h1 h2. destruct h2. 
+        destruct (progress _ _ h1); eauto.
+        intros T h1 h2; destruct h2.
+        pose (preservation _ _ _ h1 H).
+        eauto.
+Qed.
+
+
+        
+
+
+    
 
 
 
+
+
+
+
+    
+    
